src/GoCompilationLemmas.v
@@ -367,6 +367,7 @@ Proof.
   destruct a; econstructor; eauto.
 Qed.
 
+
 Lemma CompileVar : forall env A var T (v : T) {H : GoWrapper T},
   EXTRACT Ret v
   {{ var ~> v * A }}
@@ -1173,185 +1174,6 @@ Proof.
   repeat econstructor.
   all: eval_expr; [reflexivity].
 Qed.
-
-Definition middle_immut : forall low mid high w, immut_word mid := Rec.middle.
-
-Fixpoint go_rec_type (t : Rec.type) : type :=
-  match t with
-  | Rec.WordF n => ImmutableBuffer
-  | Rec.ArrayF t' n => Slice (go_rec_type t')
-  | Rec.RecF fs =>
-    (fix rec_type fs :=
-       match fs with
-       | [] => Struct []
-       | (_, f) :: fs' => Pair (go_rec_type f) (rec_type fs')
-       end) fs
-  end.
-
-Instance GoWrapper_rec t : GoWrapper (Rec.data t).
-  einduction t using Rec.type_rect_nest; simpl.
-  - change word with immut_word. typeclasses eauto.
-  - typeclasses eauto.
-  - apply IHt0.
-  - simpl; typeclasses eauto.
-  - simpl in *; typeclasses eauto.
-Defined.
-
-Lemma GoWrapper_rec_go_rec_type : forall t, @wrap_type _ (GoWrapper_rec t) = go_rec_type t.
-Proof.
-  einduction t using Rec.type_rect_nest; simpl; auto.
-  - rewrite <- IHt0; reflexivity.
-  - apply IHt0.
-  - reflexivity.
-  - simpl in *.
-    rewrite <- IHt0.
-    rewrite <- IHt1.
-    reflexivity.
-Qed.
-
-Fixpoint go_of_word (t : Rec.type) (vdst vsrc : var) (from : nat) : stmt :=
-  match t with
-  | Rec.WordF n =>
-    Declare Num (fun vfrom =>
-      Declare Num (fun vto =>
-        (Modify (@SetConst Num from) ^(vfrom); Modify (@SetConst Num (from + n)) ^(vto);
-         Modify SliceBuffer ^(vdst, vsrc, vfrom, vto))))
-  | Rec.ArrayF t' n =>
-    (fix array_of_word n from :=
-       match n with
-       | O => Modify (@SetConst (Slice (go_rec_type t')) (Here [])) ^(vdst)
-       | S n' =>
-         Declare (go_rec_type t') (fun vt' =>
-           (array_of_word n' from;
-            go_of_word t' vt' vsrc from;
-            Modify AppendOp ^(vdst, vt')))
-       end) n from
-  | Rec.RecF fs =>
-    (fix rec_of_word fs vdst from :=
-       match fs with
-       | [] => Modify (@SetConst (Struct []) tt) ^(vdst)
-       | (_, f) :: fs' =>
-         Declare (go_rec_type f) (fun vf =>
-           Declare (go_rec_type (Rec.RecF fs')) (fun vfs' =>
-             (go_of_word f vf vsrc from;
-              rec_of_word fs' vfs' (from + Rec.len f);
-              Modify JoinPair ^(vdst, vf, vfs')
-              )))
-       end) fs vdst from
-  end%go.
-
-Hint Constructors source_stmt. 
-Lemma source_stmt_go_of_word : forall t vsrc vdst from,
-    source_stmt (go_of_word t vdst vsrc from).
-Proof.
-  intros t vsrc.
-  induction t using Rec.type_rect_nest
-  with (Q := fun rt =>
-               forall vdst from, source_stmt ((fix rec_of_word fs vdst from :=
-       match fs with
-       | [] => Modify (@SetConst (Struct []) tt) ^(vdst)
-       | (_, f) :: fs' =>
-         Declare (go_rec_type f) (fun vf =>
-           Declare (go_rec_type (Rec.RecF fs')) (fun vfs' =>
-             (go_of_word f vf vsrc from;
-              rec_of_word fs' vfs' (from + Rec.len f);
-              Modify JoinPair ^(vdst, vf, vfs')
-              )))%go
-       end) rt vdst from)); simpl; intros.
-  - eauto.
-  - induction n; eauto.
-  - eapply IHt.
-  - eauto.
-  - eauto.
-Qed.
-
-Require Import PeanoNat.
-
-Fixpoint byte_aligned (t : Rec.type) : Prop :=
-  match t with
-  | Rec.WordF n => Nat.divide 8 n
-  | Rec.ArrayF t' n => byte_aligned t'
-  | Rec.RecF fs =>
-    (fix fields_aligned fs :=
-       match fs with
-       | [] => True
-       | (_, f) :: fs' =>
-         byte_aligned f /\ fields_aligned fs'
-       end) fs
-  end%go.
-
-Lemma compile_of_word' : forall (t : Rec.type) (vdst vsrc : var) before after (buf : immut_word (before + (Rec.len t + after))) env F,
-    byte_aligned t ->
-    Nat.divide 8 before ->
-    Nat.divide 8 after ->
-    EXTRACT Ret (@Rec.of_word_middle t before after buf)
-    {{ vdst ~>? Rec.data t * vsrc ~> buf * F }}
-      go_of_word t vdst vsrc before
-    {{ fun ret => vdst ~> ret * vsrc ~> buf * F }} // env.
-Proof.
-  einduction t using Rec.type_rect_nest; simpl; intros.
-  - pose proof (@CompileDeclare env (word n) nat _) as Hc.
-    eapply Hc; intros.
-    eapply Hc; intros.
-    eapply hoare_weaken.
-    eapply CompileBefore.
-    eapply hoare_weaken; [ let H' := fresh in pose proof (@CompileConst' nat _ env) as H'; eapply H' | cancel_go.. ].
-    2: cancel_go.
-    2: cancel_go.
-    eapply CompileBefore.
-    eapply hoare_weaken; [ let H' := fresh in pose proof (@CompileConst' nat _ env) as H'; eapply H' | cancel_go.. ].
-    fold plus.
-    eapply hoare_weaken; [ eapply CompileMiddle; eauto | cancel_go.. ].
-  - induction n; simpl.
-    + eapply hoare_weaken.
-      evar (F' : pred).
-      pose proof (@CompileConst (list (Rec.data t0)) _ env F' vdst []).
-      subst F'.
-      simpl in H2.
-      rewrite GoWrapper_rec_go_rec_type in H2.
-      apply H2.
-      rewrite GoWrapper_rec_go_rec_type. cancel_go.
-      cancel_go.
-    + eapply hoare_weaken. rewrite <- GoWrapper_rec_go_rec_type. eapply CompileDeclare; intros.
-    eapply extract_equiv_prog.
-    match goal with
-    | [ |- ProgMonad.prog_equiv _ ?pr ] =>
-      let Pr := fresh "Pr" in
-      set pr as Pr;
-      match goal with
-      | [ Pr := context[@Rec.of_word_middle ?a ?b ?c ?d] |- _ ] =>
-        pattern (@Rec.of_word_middle a b c d) in Pr
-      end
-    end.
-      subst Pr.
-      eapply bind_left_id.
-      eapply hoare_weaken.
-      eapply CompileBindRet.
-      eapply hoare_weaken.
-      rewrite GoWrapper_rec_go_rec_type.
-      eapply IHn.
-Admitted.
-
-Lemma compile_of_word : forall (t : Rec.type) (vdst vsrc : var) (buf : immut_word (Rec.len t)) env F,
-    byte_aligned t ->
-    EXTRACT Ret (@Rec.of_word t buf)
-    {{ vdst ~>? Rec.data t * vsrc ~> buf * F }}
-      go_of_word t vdst vsrc 0
-    {{ fun ret => vdst ~> ret * vsrc ~> buf * F }} // env.
-Proof.
-  intros.
-  erewrite Rec.of_word_middle_eq.
-  eapply hoare_weaken.
-  eapply compile_of_word'; try divisibility.
-  rewrite okToCancel_eq_rect_immut_word.
-  reflexivity.
-  intros; cbv beta.
-  rewrite okToCancel_eq_rect_immut_word.
-  reflexivity.
-  Unshelve.
-  eapply plus_n_O.
-Qed.
-
 
 Lemma CompileUncons :
   forall env T F G V {Wr: GoWrapper V} (lvar cvar xvar xsvar : var) (l : list V)
@@ -2422,5 +2244,369 @@ Proof.
     contradiction H3.
     repeat eexists. apply StepIfFalse. eval_expr.
 Qed.
+
+Definition middle_immut : forall low mid high w, immut_word mid := Rec.middle.
+
+Fixpoint go_rec_type (t : Rec.type) : type :=
+  match t with
+  | Rec.WordF n => ImmutableBuffer
+  | Rec.ArrayF t' n => Slice (go_rec_type t')
+  | Rec.RecF fs =>
+    (fix rec_type fs :=
+       match fs with
+       | [] => Struct []
+       | (_, f) :: fs' => Pair (go_rec_type f) (rec_type fs')
+       end) fs
+  end.
+
+Instance GoWrapper_rec t : GoWrapper (Rec.data t).
+  einduction t using Rec.type_rect_nest; simpl.
+  - change word with immut_word. typeclasses eauto.
+  - typeclasses eauto.
+  - apply IHt0.
+  - simpl; typeclasses eauto.
+  - simpl in *; typeclasses eauto.
+Defined.
+
+Lemma GoWrapper_rec_go_rec_type : forall t, @wrap_type _ (GoWrapper_rec t) = go_rec_type t.
+Proof.
+  einduction t using Rec.type_rect_nest; simpl; auto.
+  - rewrite <- IHt0; reflexivity.
+  - apply IHt0.
+  - reflexivity.
+  - simpl in *.
+    rewrite <- IHt0.
+    rewrite <- IHt1.
+    reflexivity.
+Qed.
+
+Fixpoint go_of_word (t : Rec.type) (vdst vsrc : var) (from : nat) : stmt :=
+  match t with
+  | Rec.WordF n =>
+    Declare Num (fun vfrom =>
+      Declare Num (fun vto =>
+        (Modify (@SetConst Num from) ^(vfrom); Modify (@SetConst Num (from + n)) ^(vto);
+         Modify SliceBuffer ^(vdst, vsrc, vfrom, vto))))
+  | Rec.ArrayF t' n =>
+    (fix array_of_word n from :=
+       match n with
+       | O => Modify (@SetConst (Slice (go_rec_type t')) (Here [])) ^(vdst)
+       | S n' =>
+         Declare (go_rec_type t') (fun vt' =>
+           (array_of_word n' (from + Rec.len t');
+            go_of_word t' vt' vsrc from;
+            Modify AppendOp ^(vdst, vt')))
+       end) n from
+  | Rec.RecF fs =>
+    (fix rec_of_word fs vdst from :=
+       match fs with
+       | [] => Modify (@SetConst (Struct []) tt) ^(vdst)
+       | (_, f) :: fs' =>
+         Declare (go_rec_type f) (fun vf =>
+           Declare (go_rec_type (Rec.RecF fs')) (fun vfs' =>
+             (go_of_word f vf vsrc from;
+              rec_of_word fs' vfs' (from + Rec.len f);
+              Modify JoinPair ^(vdst, vf, vfs')
+              )))
+       end) fs vdst from
+  end%go.
+
+Hint Constructors source_stmt. 
+Lemma source_stmt_go_of_word : forall t vsrc vdst from,
+    source_stmt (go_of_word t vdst vsrc from).
+Proof.
+  intros t vsrc.
+  induction t using Rec.type_rect_nest
+  with (Q := fun rt =>
+               forall vdst from, source_stmt ((fix rec_of_word fs vdst from :=
+       match fs with
+       | [] => Modify (@SetConst (Struct []) tt) ^(vdst)
+       | (_, f) :: fs' =>
+         Declare (go_rec_type f) (fun vf =>
+           Declare (go_rec_type (Rec.RecF fs')) (fun vfs' =>
+             (go_of_word f vf vsrc from;
+              rec_of_word fs' vfs' (from + Rec.len f);
+              Modify JoinPair ^(vdst, vf, vfs')
+              )))%go
+       end) rt vdst from)); simpl; intros.
+  - eauto.
+  - revert vdst from. induction n; eauto.
+    intros. econstructor; intro. econstructor. eapply (IHn vdst (from + Rec.len t)).
+    eauto.
+  - eapply IHt.
+  - eauto.
+  - eauto.
+Qed.
+
+Require Import PeanoNat.
+
+Fixpoint byte_aligned (t : Rec.type) : Prop :=
+  match t with
+  | Rec.WordF n => Nat.divide 8 n
+  | Rec.ArrayF t' n => byte_aligned t'
+  | Rec.RecF fs =>
+    (fix fields_aligned fs :=
+       match fs with
+       | [] => True
+       | (_, f) :: fs' =>
+         byte_aligned f /\ fields_aligned fs'
+       end) fs
+  end%go.
+
+Lemma byte_aligned_divide : forall t,
+    byte_aligned t -> Nat.divide 8 (Rec.len t).
+Proof.
+  einduction t using Rec.type_rect_nest; simpl; intros; divisibility.
+  - revert H. apply IHt0.
+  - simpl. divisibility.
+  - simpl in *. intuition.
+Qed.
+Hint Resolve byte_aligned_divide : divide.
+
+Lemma okToCancel_eq_rect_immut_word : forall x y p (e : x = y) var,
+    ((var ~> rew [immut_word] e in p) : pred) <=p=> (var ~> p).
+Proof.
+  intros.
+  replace (wrap (rew [immut_word] e in p)) with (wrap p).
+  reflexivity.
+  revert p.
+  rewrite e.
+  intros.
+  cbv [wrap wrap' GoWrapper_immut_word].
+  reflexivity.
+Qed.
+Hint Extern 0 (okToCancel (?var ~> ?p) (?var ~> rew [immut_word] ?e in ?p)) =>
+  apply okToCancel_eq_rect_immut_word.
+Hint Extern 0 (okToCancel (?var ~> rew [immut_word] ?e in ?p) (?var ~> ?p)) =>
+  apply okToCancel_eq_rect_immut_word.
+
+Definition eq_leibniz A B (f : A -> B) x y (e : x = y) : f x = f y.
+  destruct e.
+  reflexivity.
+Defined.
+
+Lemma eq_rect_leibniz : forall A B (f : A -> B) x y (e : x = y) P p,
+    rew [fun x0 => P (f x0)] e in p = rew [P] (eq_leibniz f e) in p.
+Proof.
+  intros.
+  destruct e.
+  reflexivity.
+Defined.
+
+
+Lemma compile_of_word' : forall (t : Rec.type) (vdst vsrc : var) before after (buf : immut_word (before + (Rec.len t + after))) env F,
+    byte_aligned t ->
+    Nat.divide 8 before ->
+    Nat.divide 8 after ->
+    EXTRACT Ret (@Rec.of_word_middle t before after buf)
+    {{ vdst ~>? Rec.data t * vsrc ~> buf * F }}
+      go_of_word t vdst vsrc before
+    {{ fun ret => vdst ~> ret * vsrc ~> buf * F }} // env.
+Proof.
+  einduction t using Rec.type_rect_nest; simpl; intros.
+  - pose proof (@CompileDeclare env (word n) nat _) as Hc.
+    eapply Hc; intros.
+    eapply Hc; intros.
+    eapply hoare_weaken.
+    eapply CompileBefore.
+    eapply hoare_weaken; [ let H' := fresh in pose proof (@CompileConst' nat _ env) as H'; eapply H' | cancel_go.. ].
+    2: cancel_go.
+    2: cancel_go.
+    eapply CompileBefore.
+    eapply hoare_weaken; [ let H' := fresh in pose proof (@CompileConst' nat _ env) as H'; eapply H' | cancel_go.. ].
+    fold plus.
+    eapply hoare_weaken; [ eapply CompileMiddle; eauto | cancel_go.. ].
+  - revert vdst before after buf H0 H1 H F.
+    induction n; simpl; intros.
+    + eapply hoare_weaken.
+      evar (F' : pred).
+      pose proof (@CompileConst (list (Rec.data t0)) _ env F' vdst []).
+      subst F'.
+      simpl in H2.
+      rewrite GoWrapper_rec_go_rec_type in H2.
+      apply H2.
+      rewrite GoWrapper_rec_go_rec_type. cancel_go.
+      cancel_go.
+    + eapply hoare_weaken. rewrite <- GoWrapper_rec_go_rec_type.
+      eapply CompileDeclare; intros.
+      2: cancel_go.
+      2: cancel_go.
+      eapply extract_equiv_prog.
+      match goal with
+      | [ |- ProgMonad.prog_equiv _ ?pr ] =>
+        let Pr := fresh "Pr" in
+        set pr as Pr;
+          match goal with
+          | [ Pr := context[?f ?before after n ?e] |- _ ] =>
+            pattern (f before after n e) in Pr
+          end
+      end.
+      subst Pr.
+      eapply bind_left_id.
+      eapply hoare_weaken; [ eapply CompileBindRet with (vara := vdst) | cancel_go.. ].
+      Focus 3.
+      norm.
+      do 2 delay_one.
+      eapply cancel_one.
+      eapply PickFirst.
+      reflexivity.
+      cbv [stars app pred_fold_left fold_left].
+      reflexivity.
+      eapply hoare_weaken.
+      rewrite GoWrapper_rec_go_rec_type.
+      specialize (IHn vdst (before + Rec.len t0)).
+      eapply IHn; eauto.
+      divisibility.
+
+      norm.
+      eapply cancel_one.
+      eapply PickFirst.
+      reflexivity.
+      cbv [stars app pred_fold_left fold_left].
+      cancel_go.
+      rewrite okToCancel_eq_rect_immut_word.
+      cancel_go.
+      cancel_go.
+
+      eapply extract_equiv_prog.
+      match goal with
+      | [ |- ProgMonad.prog_equiv _ ?pr ] =>
+        let Pr := fresh "Pr" in
+        set pr as Pr;
+          match goal with
+          | [ Pr := context[@Rec.of_word_middle ?a ?b ?c ?d] |- _ ] =>
+            pattern (@Rec.of_word_middle a b c d) in Pr
+          end
+      end.
+      subst Pr.
+      eapply bind_left_id.
+      eapply hoare_weaken; [ eapply CompileBindRet with (vara := var0) | cancel_go.. ].
+      eapply hoare_weaken.
+      eapply IHt0; eauto.
+      divisibility.
+      rewrite eq_rect_leibniz with (e := Rec.of_word_middle_subproof t0 after n).
+      rewrite ?okToCancel_eq_rect_immut_word.
+      cancel_go.
+      cancel_go.
+
+      eapply hoare_weaken.
+      eapply CompileAppend.
+      cancel_go.
+      intros.
+      rewrite eq_rect_leibniz with (e := Rec.of_word_middle_subproof t0 after n).
+      rewrite okToCancel_eq_rect_immut_word.
+      cancel_go.
+
+  - revert vdst vsrc before after buf env F H H0 H1. eapply IHt0.
+  - simpl; intros.
+    eapply hoare_weaken; [ eapply CompileConst with (Wr := GoWrapper_unit) | cancel_go.. ].
+  - simpl; intros.
+    
+    eapply hoare_weaken. rewrite <- GoWrapper_rec_go_rec_type.
+    eapply CompileDeclare; intros.
+    2: cancel_go.
+    2: cancel_go.
+
+    eapply hoare_weaken.
+    match goal with
+    | |- context[Declare (?f rt)] => change (f rt) with (go_rec_type (Rec.RecF rt))
+    end.
+    rewrite <- GoWrapper_rec_go_rec_type.
+    eapply CompileDeclare; intros.
+    2: cancel_go.
+    2: cancel_go.
+
+    eapply extract_equiv_prog.
+    match goal with
+    | [ |- ProgMonad.prog_equiv _ ?pr ] =>
+      let Pr := fresh "Pr" in
+      set pr as Pr;
+        match goal with
+        | [ Pr := context[@Rec.of_word_middle ?a ?b ?c ?d] |- _ ] =>
+          pattern (@Rec.of_word_middle a b c d) in Pr
+        end
+    end.
+    subst Pr.
+    eapply bind_left_id.
+    eapply hoare_weaken; [ eapply CompileBindRet with (vara := var0) | cancel_go.. ].
+    eapply hoare_weaken.
+    eapply IHt0; intuition eauto.
+    apply Nat.divide_add_r; divisibility.
+    revert H2 H3.
+    clear.
+    induction rt; [ intros; divisibility | intros; destruct a; intuition divisibility ].
+    rewrite eq_rect_leibniz with (e := Rec.of_word_middle_subproof1 after rt n t0).
+    rewrite ?okToCancel_eq_rect_immut_word.
+    cancel_go.
+    cancel_go.
+
+    eapply extract_equiv_prog.
+    match goal with
+    | [ |- ProgMonad.prog_equiv _ ?pr ] =>
+      let Pr := fresh "Pr" in
+      set pr as Pr;
+        match goal with
+        | [ Pr := context[?f ?before after rt ?e] |- _ ] =>
+          pattern (f before after rt e) in Pr
+        end
+    end.
+    subst Pr.
+    eapply bind_left_id.
+    eapply hoare_weaken; [ eapply CompileBindRet with (vara := var1) | cancel_go.. ].
+    eapply hoare_weaken.
+    cbv beta in IHt1.
+    specialize (IHt1 var1 vsrc).
+    eapply IHt1; intuition eauto.
+    divisibility.
+
+    norm.
+    eapply cancel_one.
+    eapply PickFirst.
+    reflexivity.
+    cbv [stars app pred_fold_left fold_left].
+    rewrite eq_rect_leibniz with (e := Rec.of_word_middle_subproof1 after rt n t0).
+    rewrite ?okToCancel_eq_rect_immut_word.
+    cancel_go.
+    cancel_go.
+
+
+    eapply hoare_weaken.
+    eapply CompileJoin.
+    rewrite eq_rect_leibniz with (e := Rec.of_word_middle_subproof1 after rt n t0).
+    cancel_go.
+    rewrite okToCancel_eq_rect_immut_word.
+    rewrite ?GoWrapper_rec_go_rec_type.
+    cancel_go.
+    norm.
+    do 2 delay_one.
+    eapply cancel_one.
+    eapply PickFirst.
+    reflexivity.
+    cbv [stars app pred_fold_left fold_left].
+    reflexivity.
+
+    cancel_go.
+Qed.
+
+Lemma compile_of_word : forall (t : Rec.type) (vdst vsrc : var) (buf : immut_word (Rec.len t)) env F,
+    byte_aligned t ->
+    EXTRACT Ret (@Rec.of_word t buf)
+    {{ vdst ~>? Rec.data t * vsrc ~> buf * F }}
+      go_of_word t vdst vsrc 0
+    {{ fun ret => vdst ~> ret * vsrc ~> buf * F }} // env.
+Proof.
+  intros.
+  erewrite Rec.of_word_middle_eq.
+  eapply hoare_weaken.
+  eapply compile_of_word'; try divisibility.
+  rewrite okToCancel_eq_rect_immut_word.
+  reflexivity.
+  intros; cbv beta.
+  rewrite okToCancel_eq_rect_immut_word.
+  reflexivity.
+  Unshelve.
+  eapply plus_n_O.
+Qed.
+
 
 Arguments nth_var : simpl never.
